Boundaries.v
@@ -23,63 +23,59 @@ Ltac invc_sval := _sval invc.
 (* ------------------------------------------------------------------------- *)
 
 Inductive safe_boundaries : tm -> Prop :=
-  | sb_unit  :                  safe_boundaries <{unit      }>
-
-  | sb_nat   : forall n,        safe_boundaries <{nat n     }>
-
-  | sb_var   : forall x,        safe_boundaries <{var x     }>
-
+  | sb_unit  :                  safe_boundaries <{unit         }>
+  | sb_nat   : forall n,        safe_boundaries <{nat n        }>
+  | sb_var   : forall x,        safe_boundaries <{var x        }>
   | sb_fun   : forall x Tx t,   safe_boundaries t  ->
-                                safe_boundaries <{fn x Tx t }>
-
+                                safe_boundaries <{fn x Tx t    }>
   | sb_call  : forall t1 t2,    safe_boundaries t1 ->
                                 safe_boundaries t2 ->
-                                safe_boundaries <{call t1 t2}>
-
-  | sb_ref   : forall ad T,     safe_boundaries <{&ad : T   }>
-
-  | sb_new   : forall T t,      safe_boundaries t  ->
-                                safe_boundaries <{new t : T }>
-
+                                safe_boundaries <{call t1 t2   }>
+  | sb_ref   : forall ad T,     safe_boundaries <{&ad : T      }>
+  | sb_newR   : forall t T,     safe_boundaries t  ->
+                                safe_boundaries <{new t : r&T  }>
+  | sb_newX   : forall t T,     no_wrefs t         ->
+                                safe_boundaries t  ->
+                                safe_boundaries <{new t : x&T  }>
+  | sb_newW   : forall t T,     safe_boundaries t  ->
+                                safe_boundaries <{new t : w&T  }>
+  | sb_init  : forall ad t T,   safe_boundaries t  ->
+                                safe_boundaries <{init ad t : T}>
   | sb_load  : forall t,        safe_boundaries t  ->
-                                safe_boundaries <{*t        }>
-
+                                safe_boundaries <{*t           }>
   | sb_asg   : forall t1 t2,    safe_boundaries t1 ->
                                 safe_boundaries t2 ->
-                                safe_boundaries <{t1 := t2  }>
-
+                                safe_boundaries <{t1 := t2     }>
   | sb_acq   : forall t1 t2,    safe_boundaries t1 ->
                                 safe_boundaries t2 ->
-                                safe_boundaries <{acq t1 t2 }>
-
+                                safe_boundaries <{acq t1 t2    }>
   | sb_cr1   : forall ad t,     ~ value t          ->
                                 safe_boundaries t  ->
-                                safe_boundaries <{cr ad t   }>
-
+                                safe_boundaries <{cr ad t      }>
   | sb_cr2   : forall ad t,     value t            ->
                                 safe_value t       ->
-                                safe_boundaries <{cr ad t   }>
-
+                                safe_boundaries <{cr ad t      }>
   | sb_spawn : forall t,        safe_boundaries t  ->
-                                safe_boundaries <{spawn t   }>
+                                safe_boundaries <{spawn t      }>
   .
 
 (* inversion --------------------------------------------------------------- *)
 
 Local Ltac _sb tt :=
   match goal with
-  | H : safe_boundaries <{unit     }>   |- _ => clear H
-  | H : safe_boundaries <{nat _    }>   |- _ => clear H
-  | H : safe_boundaries <{var _    }>   |- _ => clear H
-  | H : safe_boundaries <{fn _ _ _ }>   |- _ => tt H
-  | H : safe_boundaries <{call _ _ }>   |- _ => tt H
-  | H : safe_boundaries <{& _ : _  }>   |- _ => clear H
-  | H : safe_boundaries <{new _ : _}>   |- _ => tt H
-  | H : safe_boundaries <{* _      }>   |- _ => tt H
-  | H : safe_boundaries <{_ := _   }>   |- _ => tt H
-  | H : safe_boundaries <{acq _  _ }>   |- _ => tt H
-  | H : safe_boundaries <{cr _ _   }>   |- _ => tt H
-  | H : safe_boundaries <{spawn _  }>   |- _ => tt H
+  | H : safe_boundaries <{unit        }>   |- _ => clear H
+  | H : safe_boundaries <{nat _       }>   |- _ => clear H
+  | H : safe_boundaries <{var _       }>   |- _ => clear H
+  | H : safe_boundaries <{fn _ _ _    }>   |- _ => tt H
+  | H : safe_boundaries <{call _ _    }>   |- _ => tt H
+  | H : safe_boundaries <{& _ : _     }>   |- _ => clear H
+  | H : safe_boundaries <{new _ : _   }>   |- _ => tt H
+  | H : safe_boundaries <{init _ _ : _}>   |- _ => tt H
+  | H : safe_boundaries <{* _         }>   |- _ => tt H
+  | H : safe_boundaries <{_ := _      }>   |- _ => tt H
+  | H : safe_boundaries <{acq _  _    }>   |- _ => tt H
+  | H : safe_boundaries <{cr _ _      }>   |- _ => tt H
+  | H : safe_boundaries <{spawn _     }>   |- _ => tt H
   end.
 
 Ltac inv_sb  := _sb inv.
