Boundaries1.v
@@ -1,0 +1,67 @@
+From Elo Require Import Core.
+
+From Elo Require Import Properties.
+
+(* ------------------------------------------------------------------------- *)
+(* safe-newx                                                                 *)
+(* ------------------------------------------------------------------------- *)
+
+Inductive safe_newx : tm -> Prop :=
+  | snx_unit  :                safe_newx <{unit         }>
+  | snx_nat   : forall n,      safe_newx <{nat n        }>
+  | snx_var   : forall x,      safe_newx <{var x        }>
+  | snx_fun   : forall x Tx t, safe_newx t  ->
+                               safe_newx <{fn x Tx t    }>
+  | snx_call  : forall t1 t2,  safe_newx t1 ->
+                               safe_newx t2 ->
+                               safe_newx <{call t1 t2   }>
+  | snx_ref   : forall ad T,   safe_newx <{&ad : T      }>
+  | snx_newR   : forall t T,   safe_newx t  ->
+                               safe_newx <{new t : r&T  }>
+  | snx_newX   : forall t T,   no_wrefs t         ->
+                               safe_newx t  ->
+                               safe_newx <{new t : x&T  }>
+  | snx_newW   : forall t T,   safe_newx t  ->
+                               safe_newx <{new t : w&T  }>
+  | snx_init  : forall ad t T, safe_newx t  ->
+                               safe_newx <{init ad t : T}>
+  | snx_load  : forall t,      safe_newx t  ->
+                               safe_newx <{*t           }>
+  | snx_asg   : forall t1 t2,  safe_newx t1 ->
+                               safe_newx t2 ->
+                               safe_newx <{t1 := t2     }>
+  | snx_acq   : forall t1 t2,  safe_newx t1 ->
+                               safe_newx t2 ->
+                               safe_newx <{acq t1 t2    }>
+  | snx_cr    : forall ad t,   safe_newx t  ->
+                               safe_newx <{cr ad t      }>
+  | snx_spawn : forall t,      safe_newx t  ->
+                               safe_newx <{spawn t      }>
+  .
+
+(* inversion --------------------------------------------------------------- *)
+
+Local Ltac _snx tt :=
+  match goal with
+  | H : safe_newx <{unit        }>   |- _ => clear H
+  | H : safe_newx <{nat _       }>   |- _ => clear H
+  | H : safe_newx <{var _       }>   |- _ => clear H
+  | H : safe_newx <{fn _ _ _    }>   |- _ => tt H
+  | H : safe_newx <{call _ _    }>   |- _ => tt H
+  | H : safe_newx <{& _ : _     }>   |- _ => clear H
+  | H : safe_newx <{new _ : _   }>   |- _ => tt H
+  | H : safe_newx <{init _ _ : _}>   |- _ => tt H
+  | H : safe_newx <{* _         }>   |- _ => tt H
+  | H : safe_newx <{_ := _      }>   |- _ => tt H
+  | H : safe_newx <{acq _  _    }>   |- _ => tt H
+  | H : safe_newx <{cr _ _      }>   |- _ => tt H
+  | H : safe_newx <{spawn _     }>   |- _ => tt H
+  end.
+
+Ltac inv_snx  := _snx inv.
+Ltac invc_snx := _snx invc.
+
+(* preservation ------------------------------------------------------------ *)
+
+(* TODO *)
+
