NotAccess.v
@@ -1,116 +1,190 @@
+From Elo Require Import Core.
 
+From Elo Require Import AccessCore.
 
 (* ------------------------------------------------------------------------- *)
-(* not-write-access inversion                                                *)
+(* not-access                                                                *)
 (* ------------------------------------------------------------------------- *)
 
-Local Lemma inv_nwacc_ref_eq : forall m ad T,
-  ~ write_access ad m <{&ad : w&T}> ->
-  False.
-Proof. eauto using write_access. Qed.
+Local Ltac solve_cons_nacc := 
+  intros ** ?; invc_acc; try invc_eq; eauto.
 
-Local Lemma inv_nuacc_ref_neqW : forall m ad ad' T,
-  ~ write_access ad m <{&ad' : w&T}> ->
-  (ad <> ad' /\ ~ write_access ad m m[ad'].t).
+Lemma nacc_unit : forall ad m,
+  ~ access ad m <{unit}>.
+Proof. solve_cons_nacc. Qed.
+
+Lemma nacc_nat : forall ad m n,
+  ~ access ad m <{nat n}>.
+Proof. solve_cons_nacc. Qed.
+
+Lemma nacc_var : forall ad m x,
+  ~ access ad m <{var x}>.
+Proof. solve_cons_nacc. Qed.
+
+Lemma nacc_fun : forall ad m x Tx t,
+  ~ access ad m t ->
+  ~ access ad m <{fn x Tx t}>.
+Proof. solve_cons_nacc. Qed.
+
+Lemma nacc_call : forall ad m t1 t2,
+  ~ access ad m t1 ->
+  ~ access ad m t2 ->
+  ~ access ad m <{call t1 t2}>.
+Proof. solve_cons_nacc. Qed.
+
+Lemma nacc_refR : forall m ad ad' t T,
+  ad <> ad' ->
+  m[ad'].t = Some t ->
+  ~ access ad m t ->
+  ~ access ad m <{&ad' : r&T}>.
+Proof. solve_cons_nacc. Qed.
+
+Lemma nacc_refX : forall m ad ad' T,
+  ~ access ad m <{&ad' : x&T}>.
+Proof. solve_cons_nacc. Qed.
+
+Lemma nacc_refW : forall m ad ad' t T,
+  ad <> ad' ->
+  m[ad'].t = Some t ->
+  ~ access ad m t ->
+  ~ access ad m <{&ad' : w&T}>.
+Proof. solve_cons_nacc. Qed.
+
+Lemma nacc_new : forall ad m t T,
+  ~ access ad m t ->
+  ~ access ad m <{new t : T}>.
+Proof. solve_cons_nacc. Qed.
+
+Lemma nacc_initR : forall adx ad m t T,
+  ~ access ad m t ->
+  ~ access ad m <{init adx t : r&T}>.
+Proof. solve_cons_nacc. Qed.
+
+Lemma nacc_initX : forall adx ad m t T,
+  ~ access ad m <{init adx t : x&T}>.
+Proof. solve_cons_nacc. Qed.
+
+Lemma nacc_initW : forall adx ad m t T,
+  ~ access ad m t ->
+  ~ access ad m <{init adx t : w&T}>.
+Proof. solve_cons_nacc. Qed.
+
+Lemma nacc_load : forall ad m t,
+  ~ access ad m t ->
+  ~ access ad m <{*t}>.
+Proof. solve_cons_nacc. Qed.
+
+Lemma nacc_asg : forall ad m t1 t2,
+  ~ access ad m t1 ->
+  ~ access ad m t2 ->
+  ~ access ad m <{t1 := t2}>.
+Proof. solve_cons_nacc. Qed.
+
+Lemma nacc_acq : forall ad m t1 t2,
+  ~ access ad m t1 ->
+  ~ access ad m t2 ->
+  ~ access ad m <{acq t1 t2}>.
+Proof. solve_cons_nacc. Qed.
+
+Lemma nacc_cr : forall ad m adx t,
+  ~ access ad m <{cr adx t}>.
+Proof. solve_cons_nacc. Qed.
+
+Lemma nacc_spawn : forall ad m t,
+  ~ access ad m <{spawn t}>.
+Proof. solve_cons_nacc. Qed.
+
+#[export] Hint Resolve
+  nacc_unit  nacc_nat
+  nacc_var   nacc_fun   nacc_call
+  nacc_refR  nacc_refX  nacc_refW
+  nacc_new   nacc_load  nacc_asg
+  nacc_initR nacc_initX nacc_initW
+  nacc_acq   nacc_cr
+  nacc_spawn
+  : not_access.
+
+(* inversion --------------------------------------------------------------- *)
+
+Local Ltac solve_inv_nacc := 
+  intros; try split; eauto using access.
+
+Local Lemma inv_nacc_fun : forall m x Tx t ad,
+  ~ access ad m <{fn x Tx t}> ->
+  ~ access ad m t.
+Proof. solve_inv_nacc. Qed.
+
+Local Lemma inv_nacc_call : forall m t1 t2 ad,
+  ~ access ad m <{call t1 t2}> ->
+  ~ access ad m t1 /\ ~ access ad m t2.
+Proof. solve_inv_nacc. Qed.
+
+Local Lemma inv_nacc_refR : forall m ad ad' T,
+  ~ access ad m <{&ad' : r&T}> ->
+  ad <> ad' /\ (forall t, m[ad'].t = Some t -> ~ access ad m t).
 Proof.
-  intros. destruct (nat_eq_dec ad ad'); subst; eauto using write_access.
-  exfalso. eauto using inv_nwacc_ref_eq.
+  intros. assert (ad <> ad') by (intros ?; subst; eauto using access).
+  split; eauto using access.
 Qed.
 
-Lemma inv_nuacc_ref_neqI : forall m ad ad' T,
-  forall_memory m value ->
-  valid_references m <{&ad' : r&T}> ->
-  (* --- *)
-  ~ write_access ad m <{&ad' : r&T}> ->
-  ~ write_access ad m m[ad'].t.
+Local Lemma inv_nacc_refW : forall m ad ad' T,
+  ~ access ad m <{&ad' : w&T}> ->
+  ad <> ad' /\ (forall t, m[ad'].t = Some t -> ~ access ad m t).
 Proof.
-  intros * Hval **. invc_vr. intros ?.
-  specialize (Hval ad'); simpl in *.
-  destruct Hval; inv_typeof; inv_wacc; eauto.
+  intros. assert (ad <> ad') by (intros ?; subst; eauto using access).
+  split; eauto using access.
 Qed.
 
-Local Ltac solve_nuacc_inversion :=
-  intros; try (split; intros); eauto using write_access.
+Local Lemma inv_nacc_new : forall m t ad T,
+  ~ access ad m <{new t : T}> ->
+  ~ access ad m t.
+Proof. solve_inv_nacc. Qed.
 
-Local Ltac solve_nwacc_inversion :=
-  intros; try (split; intros); eauto using write_access.
+Local Lemma inv_nacc_initR : forall m ad ad' t T,
+  ~ access ad m <{init ad' t : r&T}> ->
+  ~ access ad m t.
+Proof. solve_inv_nacc. Qed.
 
-Local Lemma inv_nwacc_fun : forall m t ad x Tx,
-  ~ write_access ad m <{fn x Tx t}> ->
-  ~ write_access ad m t.
-Proof. solve_nwacc_inversion. Qed.
+Local Lemma inv_nacc_initW : forall m ad ad' t T,
+  ~ access ad m <{init ad' t : w&T}> ->
+  ~ access ad m t.
+Proof. solve_inv_nacc. Qed.
 
-Local Lemma inv_nwacc_call : forall m t1 t2 ad,
-  ~ write_access ad m <{call t1 t2}> ->
-  ~ write_access ad m t1 /\ ~ write_access ad m t2.
-Proof. solve_nwacc_inversion. Qed.
+Local Lemma inv_nacc_load : forall m t ad,
+  ~ access ad m <{*t}> ->
+  ~ access ad m t.
+Proof. solve_inv_nacc. Qed.
 
-Local Lemma inv_nwacc_ref : forall m ad T,
-  ~ write_access ad m <{&ad :: u&T}> ->
-  False.
-Proof. solve_nwacc_inversion. Qed.
+Local Lemma inv_nacc_asg : forall m t1 t2 ad,
+  ~ access ad m <{t1 := t2}> ->
+  ~ access ad m t1 /\ ~ access ad m t2.
+Proof. solve_inv_nacc. Qed.
 
-Local Lemma inv_nwacc_new : forall m t ad T,
-  ~ write_access ad m <{new T t}> ->
-  ~ write_access ad m t.
-Proof. solve_nwacc_inversion. Qed.
+Local Lemma inv_nacc_acq : forall m t1 t2 ad,
+  ~ access ad m <{acq t1 t2}> ->
+  ~ access ad m t1 /\ ~ access ad m t2.
+Proof. solve_inv_nacc. Qed.
 
-Local Lemma inv_nwacc_load : forall m t ad,
-  ~ write_access ad m <{*t}> ->
-  ~ write_access ad m t.
-Proof. solve_nwacc_inversion. Qed.
-
-Local Lemma inv_nwacc_asg : forall m t1 t2 ad,
-  ~ write_access ad m <{t1 = t2}> ->
-  ~ write_access ad m t1 /\ ~ write_access ad m t2.
-Proof. solve_nwacc_inversion. Qed.
-
-Local Lemma inv_nwacc_acq : forall m t1 t2 ad,
-  ~ write_access ad m <{acq t1 t2}> ->
-  ~ write_access ad m t1 /\ ~ write_access ad m t2.
-Proof. solve_nwacc_inversion. Qed.
-
-Local Lemma inv_nwacc_cr : forall m t ad ad',
-  ~ write_access ad m <{cr ad' t}> ->
-  ~ write_access ad m t.
-Proof. solve_nwacc_inversion. Qed.
-
-Local Lemma inv_nwacc_ptm : forall m t ad tid,
-  ~ write_access ad m <{ptm tid t}> ->
-  ~ write_access ad m t.
-Proof. solve_nwacc_inversion. Qed.
-
-Local Notation wacc := (write_access).
-
-Ltac inv_nwacc :=
-  match goal with
-  | H : ~ wacc _ _ <{unit    }> |- _ => clear H
-  | H : ~ wacc _ _ <{nat _   }> |- _ => clear H
-  | H : ~ wacc _ _ <{var _   }> |- _ => clear H
-  | H : ~ wacc _ _ <{fn _ _ _}> |- _ => eapply inv_nwacc_fun  in H
-  | H : ~ wacc _ _ <{call _ _}> |- _ => eapply inv_nwacc_call in H as [? ?]
-  | H : ~ wacc _ _ <{new _ _ }> |- _ => eapply inv_nwacc_new  in H
-  | H : ~ wacc _ _ <{* _     }> |- _ => eapply inv_nwacc_load in H
-  | H : ~ wacc _ _ <{_ = _   }> |- _ => eapply inv_nwacc_asg  in H as [? ?]
-  | H : ~ wacc _ _ <{acq _ _ }> |- _ => eapply inv_nwacc_acq  in H as [? ?]
-  | H : ~ wacc _ _ <{cr _ _  }> |- _ => eapply inv_nwacc_cr   in H
-  | H : ~ wacc _ _ <{ptm _ _ }> |- _ => eapply inv_nwacc_ptm  in H
-
-  | H : ~ wacc ?ad _ <{& ?ad :: u&_}>   |- _ => eapply inv_nwacc_ref in H;
-                                                solve contradiction
-  end.
-
-Ltac inv_nuacc :=
-  match goal with
-  | H : ~ write_access ?ad _ <{& ?ad  :: & _ }> |- _ =>
-    eapply inv_nuacc_ref_eq   in H; solve contradiction
-  | H : ~ write_access ?ad _ <{& ?ad' :: & _ }> |- _ =>
-    eapply inv_nuacc_ref_neqM in H as [? ?]
-  | H : ~ write_access _ _   <{new _ _       }> |- _ =>
-
-  | Hval   : forall_memory ?m value,
-    Hctr   : consistently_typed_references ?m <{& ?ad' :: (i& ?T) }>,
-    Hnuacc : ~ write_access ?ad ?m <{& ?ad' :: (i& ?T) }> |- _ =>
-    eapply (inv_nuacc_ref_neqI m ad ad' T Hval Hctr) in Hnuacc
-  end.
+Ltac invc_nacc :=
+match goal with
+| H: ~ access _ _ <{unit          }> |- _ => clear H
+| H: ~ access _ _ <{nat _         }> |- _ => clear H
+| H: ~ access _ _ <{var _         }> |- _ => clear H
+| H: ~ access _ _ <{fn _ _ _      }> |- _ => eapply inv_nacc_fun   in H
+| H: ~ access _ _ <{call _ _      }> |- _ => eapply inv_nacc_call  in H as [? ?]
+| H: ~ access _ _ <{& _ : r&_     }> |- _ => eapply inv_nacc_refR  in H as [? ?]
+| H: ~ access _ _ <{& _ : x&_     }> |- _ => clear H
+| H: ~ access _ _ <{& _ : w&_     }> |- _ => eapply inv_nacc_refW  in H as [? ?]
+| H: ~ access _ _ <{& _ : _       }> |- _ => idtac H
+| H: ~ access _ _ <{new _ : _     }> |- _ => eapply inv_nacc_new   in H
+| H: ~ access _ _ <{init _ _ : r&_}> |- _ => eapply inv_nacc_initR in H
+| H: ~ access _ _ <{init _ _ : x&_}> |- _ => clear H
+| H: ~ access _ _ <{init _ _ : w&_}> |- _ => eapply inv_nacc_initW in H
+| H: ~ access _ _ <{init _ _ : _  }> |- _ => idtac H
+| H: ~ access _ _ <{* _           }> |- _ => eapply inv_nacc_load  in H
+| H: ~ access _ _ <{_ := _        }> |- _ => eapply inv_nacc_asg   in H as [? ?]
+| H: ~ access _ _ <{acq _ _       }> |- _ => eapply inv_nacc_acq   in H as [? ?]
+| H: ~ access _ _ <{cr _ _        }> |- _ => clear H
+| H: ~ access _ _ <{spawn _       }> |- _ => clear H
+end.
 
