PointerTypes.v
@@ -1,0 +1,95 @@
+From Elo Require Import Core.
+
+From Elo Require Import Refs.
+
+(* ------------------------------------------------------------------------- *)
+(* pointer types                                                             *)
+(* ------------------------------------------------------------------------- *)
+
+Theorem ptyp_preservation : forall m1 m2 ths1 ths2 tid e ad,
+  m1 / ths1 ~~[tid, e]~~> m2 / ths2 ->
+  ad < #m1 ->
+  m1[ad].T = m2[ad].T.
+Proof.
+  intros. invc_cstep; trivial. invc_mstep; sigma; trivial; omicron; trivial.
+Qed.
+
+Lemma ptyp_wacc_correlation : forall m t ad,
+  forall_memory m value ->
+  forall_memory m (valid_addresses m) ->
+  valid_addreses m t ->
+  (* --- *)
+  access ad m t ->
+  write_access ad m t <-> (exists T, m[ad].T = `w&T`).
+Proof.
+  intros * ? Hmvr ? Hacc. split.
+  - intros Hwacc. clear Hacc. induction Hwacc; invc_vr; eauto.
+  - intros [? ?]. induction Hacc; invc_vr; eauto using write_access.
+    exfalso. eapply safe_then_nwacc; eauto.
+Qed.
+
+Corollary wacc_by_association : forall m t t' ad,
+  forall_memory m value ->
+  forall_memory m (valid_references m) ->
+  valid_references m t ->
+  valid_references m t' ->
+  (* --- *)
+  access ad m t ->
+  write_access ad m t' ->
+  write_access ad m t.
+Proof.
+  intros.
+  eapply ptyp_wacc_correlation; eauto.
+  eapply ptyp_wacc_correlation; eauto using wacc_then_acc.
+Qed.
+
+Lemma ptyp_racc_correlation : forall m t ad,
+  forall_memory m value ->
+  forall_memory m (valid_references m) ->
+  valid_references m t ->
+  (* --- *)
+  access ad m t ->
+  read_access ad m t <-> (exists T, m[ad].T = `r&T`).
+Proof.
+  intros * Hval ? ? Hacc. split; intros [? ?].
+  - induction Hacc; invc_vr; invc_nwacc; eauto using safe_then_nwacc.
+  - split; trivial. induction Hacc; intros ?; invc_vr; inv_wacc; eauto;
+    eapply IHHacc; eauto using wacc_by_association.
+Qed.
+
+Corollary racc_by_association : forall m t t' ad,
+  forall_memory m value ->
+  forall_memory m (valid_references m) ->
+  valid_references m t ->
+  valid_references m t' ->
+  (* --- *)
+  access ad m t ->
+  read_access ad m t' ->
+  read_access ad m t.
+Proof.
+  intros * ? ? ? ? ? Hracc.
+  eapply ptyp_racc_correlation; eauto.
+  duplicate Hracc Hracc'. destruct Hracc' as [? ?].
+  eapply ptyp_racc_correlation; eauto.
+Qed.
+
+Theorem ptyp_racc_wacc_contradiction : forall m1 m2 t1 t2 ad,
+  forall_memory m1 value ->
+  forall_memory m2 value ->
+  forall_memory m1 (valid_references m1) ->
+  forall_memory m2 (valid_references m2) ->
+  valid_references m1 t1 ->
+  valid_references m2 t2 ->
+  (* --- *)
+  m1[ad].T = m2[ad].T ->
+  read_access  ad m1 t1 ->
+  write_access ad m2 t2 ->
+  False.
+Proof.
+  intros until 7. intros Hracc Hwacc.
+  eapply ptyp_racc_correlation in Hracc as [? Htyp1];
+  eauto using racc_then_acc.
+  eapply ptyp_wacc_correlation in Hwacc as [? Htyp2];
+  eauto using wacc_then_acc.
+  rewrite Htyp1 in *. rewrite Htyp2 in *. discriminate.
+Qed.
