Promise.v
@@ -1,0 +1,157 @@
+From Elo Require Import Core.
+From Elo Require Import Properties.
+
+From Elo Require Import AccessCore.
+From Elo Require Import Inheritance.
+
+(* ------------------------------------------------------------------------- *)
+(* exclusivity-promise                                                       *)
+(* ------------------------------------------------------------------------- *)
+
+Definition exclusivity_promise (m : mem) (ths : threads) :=
+  forall adx ad tid1 tid2 T,
+    m[ad].T = `w&T` ->
+    xaccess adx ad m ths[tid2] ->
+    access ad m ths[tid1] ->
+    False.
+
+(* preservation ------------------------------------------------------------ *)
+
+Local Lemma ep_preservation_none : forall m ths tid t,
+  forall_threads ths valid_blocks ->
+  (* --- *)
+  exclusivity_promise m ths ->
+  ths[tid] --[e_none]--> t ->
+  exclusivity_promise m ths[tid <- t].
+Proof.
+  intros. intros until 3. repeat omicron; try solve [invc_acc || invc_xacc];
+  eauto using acc_inheritance_none, xacc_inheritance_none.
+Qed.
+
+Local Lemma noref_acc_contradiction : forall m t ad,
+  forall_memory m (no_ref ad) ->
+  no_ref ad t ->
+  access ad m t ->
+  False.
+Proof.
+  intros * ? ? H. induction H; invc_noref; eauto.
+Qed.
+
+Local Lemma noref_xacc_contradiction : forall m t adx ad,
+  forall_memory m (no_ref ad) ->
+  no_ref ad t ->
+  xaccess adx ad m t ->
+  False.
+Proof.
+  intros * ? ? H. induction H; invc_noref; eauto using noref_acc_contradiction.
+Qed.
+
+
+
+
+
+
+
+
+Lemma vad_nacc_length : forall m t,
+  forall_memory m (valid_addresses m) ->
+  valid_addresses m t ->
+  (* --- *)
+  access (#m) m t ->
+  False.
+Proof.
+  intros until 2. intros Hacc. induction Hacc; invc_vad; auto; eauto.
+Qed.
+
+Lemma vad_nxacc_length : forall adx m t,
+  forall_memory m (valid_addresses m) ->
+  valid_addresses m t ->
+  (* --- *)
+  xaccess adx (#m) m t ->
+  False.
+Proof.
+  intros until 2. intros Hxacc.
+  induction Hxacc; invc_vad; eauto using vad_nacc_length.
+Qed.
+
+Lemma xacc_noinit_nocr_contradiction : forall adx ad m t,
+  no_init adx t ->
+  no_cr   adx t ->
+  xaccess adx ad m t ->
+  False.
+Proof.
+  intros. induction t; invc_noinit; inv_nocr; invc_xacc; eauto.
+Qed.
+
+Lemma todo : forall ad m t T,
+  consistent_references m t ->
+  (* --- *)
+  m[ad].T = `w&T` ->
+  access ad m t ->
+  no_wrefs t ->
+  False.
+Proof.
+  intros * ? ? Hacc ?. induction Hacc; invc_cr; invc_nowrefs; eauto.
+  admit. (* Aqui tem que fazer as tretas de poiter type,
+  mas dessa vez sem write_access, só com m[ad].T = w&T *)
+Abort.
+
+Lemma todo : forall ad m t T1 T2,
+  m[ad].T = `w&T1` ->
+  no_cr (#m) t ->
+  one_init (#m) t ->
+  no_wrefs t ->
+  xaccess (#m) ad (m +++ (None, T2, false)) t ->
+  False.
+Proof.
+  intros * ? ? ? ? Hxacc. induction Hxacc;
+  try solve [
+    invc_nowrefs; invc_nocr; inv_oneinit;
+    eauto using xacc_noinit_nocr_contradiction
+  ].
+  invc_nowrefs. invc_nocr. invc_oneinit; eauto.
+  - invc_oneinit.
+  - 
+Abort.
+
+
+
+
+
+
+
+Local Lemma ep_preservation_alloc : forall m ths tid t T,
+  forall_threads ths (valid_addresses m) ->
+  no_uninitialized_references m ths ->
+  (* --- *)
+  exclusivity_promise m ths ->
+  ths[tid] --[e_alloc (#m) T]--> t ->
+  exclusivity_promise (m +++ (None, T, false)) ths[tid <- t].
+Proof.
+  intros * Hvad Hnur Hep Htstep.
+  assert (Hvad' : valid_addresses (m +++ (None, T, false)) t)
+    by eauto using vad_preservation_alloc.
+  assert
+    (Hnur' : no_uninitialized_references (m +++ (None, T, false)) ths[tid <- t])
+    by eauto using nur_preservation_alloc.
+  rename T into T'.
+  intros until 3. upsilon.
+  - assert (Hm : (m +++ (None, `w&T`, false))[#m].t = None) by (sigma; trivial).
+    specialize (Hnur' (#m) Hm) as [? Hths].
+    repeat omicron; try solve [invc_acc || invc_xacc].
+    + specialize (Hths tid2). sigma. eauto using noref_acc_contradiction.
+    + specialize (Hths tid1). sigma. eauto using noref_acc_contradiction.
+    + specialize (Hths tid1). sigma. eauto using noref_acc_contradiction.
+    + specialize (Hths tid1). sigma. eauto using noref_acc_contradiction.
+  - repeat omicron; try solve [invc_acc || invc_xacc].
+    + destruct (nat_eq_dec (#m) adx); subst.
+      * assert (no_init (#m) ths[tid2]) by eauto using vad_noinit_ad.
+        assert (one_init (#m) t) by eauto using noinit_to_oneinit.
+      * eauto using acc_inheritance_alloc, xacc_inheritance_alloc.
+    + eauto using acc_inheritance_alloc, xacc_inheritance_mem_add.
+    + destruct (nat_eq_dec (#m) adx); subst.
+      * admit.
+      * eauto using xacc_inheritance_alloc, acc_inheritance_mem_add.
+    + eauto using acc_inheritance_mem_add, xacc_inheritance_mem_add.
+Qed.
+
