XArea.v
@@ -1,0 +1,29 @@
+From Elo Require Import Core.
+
+From Elo Require Import Blocks.
+From Elo Require Import Inits.
+From Elo Require Import CriticalRegions.
+
+(* ------------------------------------------------------------------------- *)
+(* init-cr-exclusivity                                                       *)
+(* ------------------------------------------------------------------------- *)
+
+Definition init_cr_exclusivity (m : mem) (ths : threads) := forall ad tid1 tid2,
+  (one_init ad ths[tid1] -> no_cr   ad ths[tid2]) /\
+  (one_cr   ad ths[tid1] -> no_init ad ths[tid2]).
+
+(* preservation ------------------------------------------------------------ *)
+
+Lemma ice_preservation_none : forall m ths tid t,
+  init_cr_exclusivity m ths ->
+  ths[tid] --[e_none]--> t ->
+  init_cr_exclusivity m ths[tid <- t].
+Proof.
+  intros * Hice Htstep ad tid1 tid2.
+  specialize (Hice ad tid1 tid2) as [Hinit Hcr].
+  split; intros Hone.
+  - repeat omicron; eauto using nocr_preservation_none.
+    + eapply nocr_preservation_none; eauto. eapply Hinit. admit.
+    + eapply Hinit. admit.
+  -
+Qed.
